proof/TPOSR/Types.v
@@ -17,6 +17,8 @@ Definition sum_sort s1 s2 s3 :=
   (s1 = set /\ s2 = set /\ s3 = set) \/
   (s1 = prop /\ s2 = prop /\ s3 = prop).
 
+Reserved Notation "G |-- T ~= U : s" (at level 70, T, U, s at next level).
+
 Inductive tposr_wf : lenv -> Prop :=
   | wf_nil : tposr_wf nil
   | wf_cons : forall G A A' s, G |-- A -> A' : Srt_l s -> tposr_wf (A :: G)
@@ -83,7 +85,9 @@ with tposr : lenv -> lterm -> lterm -> lterm -> Prop :=
   forall B B' s2, (A :: e) |-- B -> B' : Srt_l s2 ->
   forall s3, sum_sort s1 s2 s3 ->
   forall u u' v v', e |-- Pair_l (Sum_l A B) u v -> Pair_l (Sum_l A' B') u' v' : Sum_l A B ->
-  e |-- Pi1_l (Sum_l A B) (Pair_l (Sum_l A B) u v) -> u : A
+  forall A'', e |-- A'' ~= A : s1 ->
+  forall B'', A'' :: e |-- B'' ~= B : s2 ->
+  e |-- Pi1_l (Sum_l A'' B'') (Pair_l (Sum_l A B) u v) -> u' : A''
 
   | tposr_pi2 : forall e A A' s1, e |-- A -> A' : Srt_l s1 ->
   forall B B' s2, (A :: e) |-- B -> B' : Srt_l s2 ->
@@ -96,9 +100,19 @@ with tposr : lenv -> lterm -> lterm -> lterm -> Prop :=
   forall s3, sum_sort s1 s2 s3 ->
   forall u u' v v', 
   e |-- Pair_l (Sum_l A B) u v -> Pair_l (Sum_l A' B') u' v' : Sum_l A B ->
-  e |-- Pi2_l (Sum_l A B) (Pair_l (Sum_l A B) u v) -> v : lsubst (Pi1_l (Sum_l A B) (Pair_l (Sum_l A B) u v)) B
+  e |-- Pi2_l (Sum_l A B) (Pair_l (Sum_l A B) u v) -> v' : lsubst (Pi1_l (Sum_l A B) (Pair_l (Sum_l A B) u v)) B
 
-where "G |-- T -> U : s" := (tposr G T U s).
+where "G |-- T -> U : s" := (tposr G T U s)
+
+with tposr_eq : lenv -> lterm -> lterm -> sort -> Prop :=
+  | tposr_eq_tposr : forall e X Y s, e |-- X -> Y : Srt_l s -> e |-- X ~= Y : s
+  | tposr_eq_sym : forall e X Y s, e |-- X ~= Y : s -> e |-- Y ~= X : s
+  | tposr_eq_trans : forall e W X Y s, e |-- W ~= X : s -> e |-- X ~= Y : s ->
+  e |-- W ~= Y : s
+
+where "G |-- T ~= U : s" := (tposr_eq G T U s).
+
+
 
 Hint Resolve wf_nil tposr_set tposr_prop : coc.
 
@@ -218,8 +232,10 @@ forall
                 : Sum_l A B),
         P e (Pair_l (Sum_l A B) u v) (Pair_l (Sum_l A' B') u' v') (Sum_l A B)
           t1 ->
-        P e (Pi1_l (Sum_l A B) (Pair_l (Sum_l A B) u v)) u A
-          (tposr_pi1_red t t0 s t1)) ->
+        forall (A'' : lterm) (t2 : e |-- A'' ~= A : s1) (B'' : lterm)
+          (t3 : A'' :: e |-- B'' ~= B : s2),
+        P e (Pi1_l (Sum_l A'' B'') (Pair_l (Sum_l A B) u v)) u' A''
+          (tposr_pi1_red t t0 s t1 t2 t3)) ->
        (forall (e : lenv) (A A' : lterm) (s1 : sort)
           (t : e |-- A -> A' : Srt_l s1),
         P e A A' (Srt_l s1) t ->
@@ -242,14 +258,13 @@ forall
                 : Sum_l A B),
         P e (Pair_l (Sum_l A B) u v) (Pair_l (Sum_l A' B') u' v') (Sum_l A B)
           t1 ->
-        P e (Pi2_l (Sum_l A B) (Pair_l (Sum_l A B) u v)) v
+        P e (Pi2_l (Sum_l A B) (Pair_l (Sum_l A B) u v)) v'
           (lsubst (Pi1_l (Sum_l A B) (Pair_l (Sum_l A B) u v)) B)
           (tposr_pi2_red t t0 s t1)) ->
        P0 nil wf_nil ->
        (forall (G : lenv) (A A' : lterm) (s : sort)
           (t : G |-- A -> A' : Srt_l s),
         P G A A' (Srt_l s) t -> P0 (A :: G) (wf_cons t)) ->
-
        (forall (l : lenv) (l0 l1 l2 : lterm) (t : l |-- l0 -> l1 : l2),
        P l l0 l1 l2 t) /\
        (forall (l : lenv) (t : tposr_wf l), P0 l t).
@@ -262,19 +277,187 @@ Proof.
   eapply wf_tposr_mutind with (P := P) (P0 := P0) ; auto ; auto.
 Qed.
 
+Scheme tposr_wf_eq_mutind := Induction for tposr Sort Prop
+with wf_tposr_eq_mutind :=  Induction for tposr_wf Sort Prop
+with eq_tposr_wf_mutind :=  Induction for tposr_eq Sort Prop.
+
+Check tposr_wf_eq_mutind.
+
+Lemma ind_tposr_wf_eq :
+forall
+         (P : forall (l : lenv) (l0 l1 l2 : lterm),
+              l |-- l0 -> l1 : l2 -> Prop)
+         (P0 : forall l : lenv, tposr_wf l -> Prop)
+         (P1 : forall (l : lenv) (l0 l1 : lterm) (s : sort),
+               l |-- l0 ~= l1 : s -> Prop),
+       (forall (e : lenv) (t : tposr_wf e),
+        P0 e t ->
+        forall (n : nat) (T : lterm) (i : item_llift T e n),
+        P e (Ref_l n) (Ref_l n) T (tposr_var t i)) ->
+       (forall (e : lenv) (t : tposr_wf e),
+        P0 e t -> P e (Srt_l set) (Srt_l set) (Srt_l kind) (tposr_set t)) ->
+       (forall (e : lenv) (t : tposr_wf e),
+        P0 e t -> P e (Srt_l prop) (Srt_l prop) (Srt_l kind) (tposr_prop t)) ->
+       (forall (e : lenv) (A A' : lterm) (s1 : sort)
+          (t : e |-- A -> A' : Srt_l s1),
+        P e A A' (Srt_l s1) t ->
+        forall (B B' : lterm) (s2 : sort)
+          (t0 : A :: e |-- B -> B' : Srt_l s2),
+        P (A :: e) B B' (Srt_l s2) t0 ->
+        P e (Prod_l A B) (Prod_l A' B') (Srt_l s2) (tposr_prod t t0)) ->
+       (forall (e : lenv) (A A' : lterm) (s1 : sort)
+          (t : e |-- A -> A' : Srt_l s1),
+        P e A A' (Srt_l s1) t ->
+        forall (B B' : lterm) (s2 : sort)
+          (t0 : A :: e |-- B -> B' : Srt_l s2),
+        P (A :: e) B B' (Srt_l s2) t0 ->
+        forall (M M' : lterm) (t1 : A :: e |-- M -> M' : B),
+        P (A :: e) M M' B t1 ->
+        P e (Abs_l A M) (Abs_l A' M') (Prod_l A B) (tposr_abs t t0 t1)) ->
+       (forall (e : lenv) (A A' : lterm) (s1 : sort)
+          (t : e |-- A -> A' : Srt_l s1),
+        P e A A' (Srt_l s1) t ->
+        forall (B B' : lterm) (s2 : sort)
+          (t0 : A :: e |-- B -> B' : Srt_l s2),
+        P (A :: e) B B' (Srt_l s2) t0 ->
+        forall (M M' : lterm) (t1 : e |-- M -> M' : Prod_l A B),
+        P e M M' (Prod_l A B) t1 ->
+        forall (N N' : lterm) (t2 : e |-- N -> N' : A),
+        P e N N' A t2 ->
+        P e (App_l B M N) (App_l B' M' N') (lsubst N B)
+          (tposr_app t t0 t1 t2)) ->
+       (forall (e : lenv) (A A' : lterm) (s1 : sort)
+          (t : e |-- A -> A' : Srt_l s1),
+        P e A A' (Srt_l s1) t ->
+        forall (B B' : lterm) (s2 : sort)
+          (t0 : A :: e |-- B -> B' : Srt_l s2),
+        P (A :: e) B B' (Srt_l s2) t0 ->
+        forall (M M' : lterm) (t1 : A :: e |-- M -> M' : B),
+        P (A :: e) M M' B t1 ->
+        forall (N N' : lterm) (t2 : e |-- N -> N' : A),
+        P e N N' A t2 ->
+        P e (App_l B (Abs_l A M) N) (lsubst N' M') (lsubst N B)
+          (tposr_beta t t0 t1 t2)) ->
+       (forall (e : lenv) (M N A : lterm) (t : e |-- M -> N : A),
+        P e M N A t ->
+        forall (B : lterm) (s : sort) (t0 : e |-- A -> B : Srt_l s),
+        P e A B (Srt_l s) t0 -> P e M N B (tposr_red t t0)) ->
+       (forall (e : lenv) (M N B : lterm) (t : e |-- M -> N : B),
+        P e M N B t ->
+        forall (A : lterm) (s : sort) (t0 : e |-- A -> B : Srt_l s),
+        P e A B (Srt_l s) t0 -> P e M N A (tposr_exp t t0)) ->
+       (forall (e : lenv) (A A' : lterm) (t : e |-- A -> A' : Srt_l set),
+        P e A A' (Srt_l set) t ->
+        forall (B B' : lterm) (t0 : A :: e |-- B -> B' : Srt_l prop),
+        P (A :: e) B B' (Srt_l prop) t0 ->
+        P e (Subset_l A B) (Subset_l A' B') (Srt_l set) (tposr_subset t t0)) ->
+       (forall (e : lenv) (A A' : lterm) (s1 : sort)
+          (t : e |-- A -> A' : Srt_l s1),
+        P e A A' (Srt_l s1) t ->
+        forall (B B' : lterm) (s2 : sort)
+          (t0 : A :: e |-- B -> B' : Srt_l s2),
+        P (A :: e) B B' (Srt_l s2) t0 ->
+        forall (s3 : sort) (s : sum_sort s1 s2 s3),
+        P e (Sum_l A B) (Sum_l A' B') (Srt_l s3) (tposr_sum t t0 s)) ->
+       (forall (e : lenv) (A A' : lterm) (s1 : sort)
+          (t : e |-- A -> A' : Srt_l s1),
+        P e A A' (Srt_l s1) t ->
+        forall (B B' : lterm) (s2 : sort)
+          (t0 : A :: e |-- B -> B' : Srt_l s2),
+        P (A :: e) B B' (Srt_l s2) t0 ->
+        forall (s3 : sort) (s : sum_sort s1 s2 s3) (u u' : lterm)
+          (t1 : e |-- u -> u' : A),
+        P e u u' A t1 ->
+        forall (v v' : lterm) (t2 : e |-- v -> v' : lsubst u B),
+        P e v v' (lsubst u B) t2 ->
+        P e (Pair_l (Sum_l A B) u v) (Pair_l (Sum_l A' B') u' v') (Sum_l A B)
+          (tposr_pair t t0 s t1 t2)) ->
+       (forall (e : lenv) (A A' : lterm) (s1 : sort)
+          (t : e |-- A -> A' : Srt_l s1),
+        P e A A' (Srt_l s1) t ->
+        forall (B B' : lterm) (s2 : sort)
+          (t0 : A :: e |-- B -> B' : Srt_l s2),
+        P (A :: e) B B' (Srt_l s2) t0 ->
+        forall (s3 : sort) (s : sum_sort s1 s2 s3) (t1 t' : lterm)
+          (t2 : e |-- t1 -> t' : Sum_l A B),
+        P e t1 t' (Sum_l A B) t2 ->
+        P e (Pi1_l (Sum_l A B) t1) (Pi1_l (Sum_l A' B') t') A
+          (tposr_pi1 t t0 s t2)) ->
+       (forall (e : lenv) (A A' : lterm) (s1 : sort)
+          (t : e |-- A -> A' : Srt_l s1),
+        P e A A' (Srt_l s1) t ->
+        forall (B B' : lterm) (s2 : sort)
+          (t0 : A :: e |-- B -> B' : Srt_l s2),
+        P (A :: e) B B' (Srt_l s2) t0 ->
+        forall (s3 : sort) (s : sum_sort s1 s2 s3) (u u' v v' : lterm)
+          (t1 : e |-- Pair_l (Sum_l A B) u v -> Pair_l (Sum_l A' B') u' v'
+                : Sum_l A B),
+        P e (Pair_l (Sum_l A B) u v) (Pair_l (Sum_l A' B') u' v') (Sum_l A B)
+          t1 ->
+        forall (A'' : lterm) (t2 : e |-- A'' ~= A : s1),
+        P1 e A'' A s1 t2 ->
+        forall (B'' : lterm) (t3 : A'' :: e |-- B'' ~= B : s2),
+        P1 (A'' :: e) B'' B s2 t3 ->
+        P e (Pi1_l (Sum_l A'' B'') (Pair_l (Sum_l A B) u v)) u' A''
+          (tposr_pi1_red t t0 s t1 t2 t3)) ->
+       (forall (e : lenv) (A A' : lterm) (s1 : sort)
+          (t : e |-- A -> A' : Srt_l s1),
+        P e A A' (Srt_l s1) t ->
+        forall (B B' : lterm) (s2 : sort)
+          (t0 : A :: e |-- B -> B' : Srt_l s2),
+        P (A :: e) B B' (Srt_l s2) t0 ->
+        forall (s3 : sort) (s : sum_sort s1 s2 s3) (t1 t' : lterm)
+          (t2 : e |-- t1 -> t' : Sum_l A B),
+        P e t1 t' (Sum_l A B) t2 ->
+        P e (Pi2_l (Sum_l A B) t1) (Pi2_l (Sum_l A' B') t')
+          (lsubst (Pi1_l (Sum_l A B) t1) B) (tposr_pi2 t t0 s t2)) ->
+       (forall (e : lenv) (A A' : lterm) (s1 : sort)
+          (t : e |-- A -> A' : Srt_l s1),
+        P e A A' (Srt_l s1) t ->
+        forall (B B' : lterm) (s2 : sort)
+          (t0 : A :: e |-- B -> B' : Srt_l s2),
+        P (A :: e) B B' (Srt_l s2) t0 ->
+        forall (s3 : sort) (s : sum_sort s1 s2 s3) (u u' v v' : lterm)
+          (t1 : e |-- Pair_l (Sum_l A B) u v -> Pair_l (Sum_l A' B') u' v'
+                : Sum_l A B),
+        P e (Pair_l (Sum_l A B) u v) (Pair_l (Sum_l A' B') u' v') (Sum_l A B)
+          t1 ->
+        P e (Pi2_l (Sum_l A B) (Pair_l (Sum_l A B) u v)) v'
+          (lsubst (Pi1_l (Sum_l A B) (Pair_l (Sum_l A B) u v)) B)
+          (tposr_pi2_red t t0 s t1)) ->
+       P0 nil wf_nil ->
+       (forall (G : lenv) (A A' : lterm) (s : sort)
+          (t : G |-- A -> A' : Srt_l s),
+        P G A A' (Srt_l s) t -> P0 (A :: G) (wf_cons t)) ->
+       (forall (e : lenv) (X Y : lterm) (s : sort)
+          (t : e |-- X -> Y : Srt_l s),
+        P e X Y (Srt_l s) t -> P1 e X Y s (tposr_eq_tposr t)) ->
+       (forall (e : lenv) (X Y : lterm) (s : sort) (t : e |-- X ~= Y : s),
+        P1 e X Y s t -> P1 e Y X s (tposr_eq_sym t)) ->
+       (forall (e : lenv) (W X Y : lterm) (s : sort) (t : e |-- W ~= X : s),
+        P1 e W X s t ->
+        forall t0 : e |-- X ~= Y : s,
+        P1 e X Y s t0 -> P1 e W Y s (tposr_eq_trans t t0)) ->
+
+       (forall (l : lenv) (l0 l1 l2 : lterm) (t : l |-- l0 -> l1 : l2),
+       P l l0 l1 l2 t) /\
+       (forall (l : lenv) (t : tposr_wf l), P0 l t) /\
+       (forall (l : lenv) (l0 l1 : lterm) (s : sort) (t : l |-- l0 ~= l1 : s),
+       P1 l l0 l1 s t).
+Proof.
+  intros.
+  split.
+  intros.
+  eapply tposr_wf_eq_mutind with (P := P) (P0 := P0) (P1 := P1); auto ; auto.
+  split ;intros.
+  eapply wf_tposr_eq_mutind with (P := P) (P0 := P0) (P1 := P1) ; auto ; auto.
+  eapply eq_tposr_wf_mutind with (P := P) (P0 := P0) (P1 := P1) ; auto ; auto.
+Qed.
+
 Inductive tposrp : lenv -> lterm -> lterm -> lterm -> Prop :=
   | tposrp_tposr : forall e X Y Z, e |-- X -> Y : Z -> tposrp e X Y Z
   | tposrp_trans : forall e W X Y Z, tposrp e W X Z -> tposrp e X Y Z ->
   tposrp e W Y Z.
 
-Reserved Notation "G |-- T ~= U : s" (at level 70, T, U, s at next level).
-
-Inductive tposr_eq : lenv -> lterm -> lterm -> sort -> Prop :=
-  | tposr_eq_tposr : forall e X Y s, e |-- X -> Y : Srt_l s -> e |-- X ~= Y : s
-  | tposr_eq_sym : forall e X Y s, e |-- X ~= Y : s -> e |-- Y ~= X : s
-  | tposr_eq_trans : forall e W X Y s, e |-- W ~= X : s -> e |-- X ~= Y : s ->
-  e |-- W ~= Y : s
-
-where "G |-- T ~= U : s" := (tposr_eq G T U s).
 
 Hint Resolve tposr_eq_tposr tposr_eq_sym : coc.
