proof/Meta/TPOSR_JRussell.v
@@ -3,6 +3,7 @@ Require Import Lambda.Reduction.
 Require Import Lambda.Conv.
 Require Import Lambda.LiftSubst.
 Require Import Lambda.Env.
+Require Import Lambda.Tactics.
 
 Require Import JRussell.Types.
 Require Import JRussell.Basic.
@@ -46,16 +47,20 @@ Theorem unlab_sound  :
   (unlab_ctx e) |-= Srt prop : Srt kind /\
   (unlab_ctx e) |-= Srt set : Srt kind /\
   (forall A n, item_llift A e n -> 
-  (unlab_ctx e) |-= Ref n : (|A|))).
+  (unlab_ctx e) |-= Ref n : (|A|))) /\
+  (forall e u v s, e |-- u ~= v : s ->
+  (unlab_ctx e) |-= (|u|) = (|v|) : Srt s).
 Proof.
-  apply ind_tposr_wf with 
+  apply ind_tposr_wf_eq with 
   (P := fun e u v T =>  fun H : e |-- u -> v : T =>
   (unlab_ctx e) |-= (|u|) = (|v|) : (|T|))
   (P0 := fun e => fun H : tposr_wf e =>
   (unlab_ctx e) |-= Srt prop : Srt kind /\
   (unlab_ctx e) |-= Srt set : Srt kind /\
   (forall A n, item_llift A e n -> 
-  (unlab_ctx e) |-= Ref n : (|A|))) ; simpl ; intros ; auto with coc.
+  (unlab_ctx e) |-= Ref n : (|A|)))
+  (P1 := fun e u v s => fun H : e |-- u ~= v : s =>
+  (unlab_ctx e) |-= (|u|) = (|v|) : Srt s) ; simpl ; intros ; auto with coc.
 
   intuition.
 
@@ -98,41 +103,78 @@ Proof.
   pose (jeq_type_l H).
   pose (jeq_type_l H0).
   pose (jeq_type_l H1).
-  pose (generation_pair t4).
-  destruct e0.
-  do 4 destruct H2.
-  intuition.
-  inversion H3.
+  pose (jeq_type_l H2).
+  pose (jeq_type_l H3).
+  pose (generation_pair t6).
+  destruct_exists.
+  pose (jeq_type_r H1).
+  inversion H4.
+  pose (generation_pair t9) ; destruct_exists.
+  apply jeq_trans with (Pi1 (Pair (Sum (|A'|) (|B'|)) (|u'|) (|v'|))) ; auto with coc.
+  apply jeq_conv with (|A|) s1 ; auto with coc.
+  apply jeq_pi1 with (|B|) ; auto with coc.
+  apply jeq_conv with (|A'|) s1 ; auto with coc.
+  inversion H11.
   apply jeq_pi1_red with s1 s2 s3 ; auto with coc.
-  rewrite H10 ; assumption.
-  rewrite H11 ; assumption.
+  apply (jeq_type_r H).
+  pose (jeq_type_r H0).
+  apply type_conv_env with ((|A|) :: unlab_ctx e) ; auto with coc.
+  apply conv_env_hd with s1 ; auto with coc.
+  rewrite H21 ; assumption.
+  rewrite H22 ; assumption.
+  apply coerce_conv ; auto.
+  apply jeq_trans with (|A|) ; auto with coc.
 
   rewrite lab_subst.
   simpl.
   apply jeq_pi2 with (|A|) ; auto with coc.
 
   pose (jeq_type_l H).
+  pose (jeq_type_r H).
   pose (jeq_type_l H0).
+  pose (jeq_type_r H0).
   pose (jeq_type_l H1).
-  pose (generation_pair t4).
-  destruct e0.
-  do 4 destruct H2.
-  intuition.
+  pose (jeq_type_r H1).
+  pose (generation_pair t6).
+  pose (generation_pair t7).
+  destruct_exists.
   inversion H3.
+  inversion H2.
   rewrite lab_subst.
-  apply jeq_conv with (subst (|u|) (|B|)) s2 ; auto with coc.
+  apply jeq_trans with (Pi2 (Pair (Sum (|A'|) (|B'|)) (|u'|) (|v'|))) ; auto with coc.
+  simpl. 
+  apply jeq_pi2 with (|A|) ; auto with coc.
+  simpl.
+  apply jeq_conv with (subst (|u'|) (|B'|)) s2 ; auto with coc.
   apply jeq_pi2_red with s1 s2 s3 ; auto with coc.
-  rewrite H10 ; assumption.
-  rewrite H11 ; assumption.
+  apply type_conv_env with ((|A|) :: unlab_ctx e) ; auto with coc.
+  apply conv_env_hd with s1 ; auto with coc.
+  rewrite H19 ; assumption.
+  rewrite H20 ; assumption.
+
   apply coerce_conv.
-  change (Srt s2) with (subst (|u|) (Srt s2)).
+  change (Srt s2) with (subst (|u'|) (Srt s2)).
+  apply jeq_trans with (subst (|u'|) (|B|)) ; auto with coc.
+  apply substitution_jeq with x ; auto with coc.
+  apply jeq_conv_env with ((|A|) :: unlab_ctx e) ; auto with coc.
+  apply conv_env_hd with s1 ; auto with coc.
+  rewrite <- H19 ; auto with coc.
   apply functionality with x ; auto with coc.
   apply jeq_sym.
   simpl.
-  rewrite <- H10 ; apply jeq_pi1_red with s1 s2 s3 ; auto with coc.
-  rewrite H10 ; auto.
-  rewrite H11 ; auto.
-  rewrite <- H10 ; auto.
+  rewrite <- H19.
+  apply jeq_conv with (|A|) s1 ; auto with coc.
+  apply jeq_trans with (Pi1 (Pair (Sum (|A'|) (|B'|)) (|u'|) (|v'|))) ; auto with coc.
+  apply jeq_pi1 with (|B|) ; auto with coc.
+  apply jeq_conv with (|A'|) s1 ; auto with coc.
+  apply jeq_pi1_red with s1 s2 s3 ; auto with coc.
+  apply type_conv_env with ((|A|) :: unlab_ctx e) ; auto with coc.
+  apply conv_env_hd with s1 ; auto with coc.
+  rewrite H19 ; assumption.
+  rewrite H20 ; assumption.
+  rewrite <- H19.
+  apply type_conv_env with ((|A|) :: unlab_ctx e) ; auto with coc.
+  apply conv_env_hd with s1 ; auto with coc.
 
   split ; auto with coc.
   split ; auto with coc.
@@ -167,6 +209,8 @@ Proof.
   apply consistent_cons with s.
   apply (jeq_consistent H).
   apply (jeq_type_l H).
+
+  apply jeq_trans with (|X|) ; auto.
 Qed.
 
 Corollary unlab_sound_type : forall e u v T, e |-- u -> v : T -> 
@@ -179,6 +223,9 @@ Corollary unlab_sound_wf :
   (unlab_ctx e) |-= Srt set : Srt kind /\
   (forall A n, item_llift A e n -> 
   (unlab_ctx e) |-= Ref n : (|A|))).
-Proof (proj2 (unlab_sound)).
+Proof (proj1 (proj2 (unlab_sound))).
 
+Corollary unlab_sound_eq : forall e u v s, e |-- u ~= v : s -> 
+  (unlab_ctx e) |-= (|u|) = (|v|) : Srt s.
+Proof (proj2 (proj2 (unlab_sound))).
 
